Clean up and organize code

Imp.lean
@@ -2,32 +2,15 @@ import Lean.PrettyPrinter.Delaborator
 import LeanSAT.Reflect.Tactics.BVDecide
 
 import Imp.Expr
-import Imp.Expr.Eval
-import Imp.Expr.Optimize
-import Imp.Expr.Delab
-
 import Imp.Stmt
-import Imp.Stmt.Delab
-import Imp.Stmt.BigStep
-import Imp.Stmt.Optimize
 
-namespace Imp
+namespace Imp.Stmt
 
-open Lean PrettyPrinter Delaborator SubExpr Parenthesizer
+open BitVec -- Enables bitvector literal syntax and lemmas
 
-open Stmt
-
-open BitVec
-
-
-def popcount : Stmt := imp {
-  x := x - ((x >>> 1) &&& 0x55555555);
-  x := (x &&& 0x33333333) + ((x >>> 2) &&& 0x33333333);
-  x := (x + (x >>> 4)) &&& 0x0F0F0F0F;
-  x := x + (x >>> 8);
-  x := x + (x >>> 16);
-  x := x &&& 0x0000003F;
-}
+/-
+The final demo - read this file last!
+-/
 
 def popcountLoop : Stmt := imp {
   i := 32;
@@ -40,8 +23,22 @@ def popcountLoop : Stmt := imp {
   x := count;
 }
 
-def pop_spec' (x : BitVec 32) : BitVec 32 :=
-  go x 0#32 32
+/--
+Alternative implementation of popcount from Hacker's Delight, Second Edition, by Henry S. Warren,
+Jr. Figure 5-2 on p. 82.
+-/
+def popcount : Stmt := imp {
+  x := x - ((x >>> 1) &&& 0x55555555);
+  x := (x &&& 0x33333333) + ((x >>> 2) &&& 0x33333333);
+  x := (x + (x >>> 4)) &&& 0x0F0F0F0F;
+  x := x + (x >>> 8);
+  x := x + (x >>> 16);
+  x := x &&& 0x0000003F;
+}
+
+
+def pop_spec (x : BitVec 32) : BitVec 32 :=
+  go x 0 32
 where
   go (x : BitVec 32) (pop : BitVec 32) (i : Nat) : BitVec 32 :=
     match i with
@@ -51,18 +48,7 @@ where
       go (x >>> 1#32) pop i
 
 
-@[simp]
-theorem Env.get_init : (Env.init v).get x = v := by rfl
-
-@[simp]
-theorem Env.get_set_same {ρ : Env} : (ρ.set x v).get x = v := by
-  simp [get, set]
-
-@[simp]
-theorem Env.get_set_different {ρ : Env} : x ≠ y → (ρ.set x v).get y = ρ.get y := by
-  intros
-  simp [get, set, *]
-
-theorem popCount_correctBig : ∃ ρ, (run' (Env.init x) popcount 8) = some ρ ∧ ρ "x" = pop_spec' x := by
-  simp [run', popcount, Expr.eval, Expr.BinOp.apply, Env.set, Value, pop_spec', pop_spec'.go]
+theorem popCount_correctBig :
+    ∃ ρ, (run (Env.init x) popcount 8) = some ρ ∧ ρ "x" = pop_spec x := by
+  simp [run, popcount, Expr.eval, Expr.BinOp.apply, Env.set, Value, pop_spec, pop_spec.go]
   bv_decide
