Imp/Stmt/BigStep.lean
@@ -1,6 +1,5 @@
 import Imp.Expr
-import Imp.Expr.Eval
-import Imp.Stmt
+
 import Imp.Stmt.Delab
 import Imp.Stmt.Optimize
 
@@ -49,9 +48,6 @@ theorem Falsy.some_zero : Falsy (some v) = (v = 0) := by
 theorem Falsy.not_none : Falsy none = False := by
   simp [Falsy]
 
-@[simp]
-theorem Falsy.some_const : Falsy (some (BitVec.ofNat _ n)) → (n % 2 ^ 32 = 0) := by
-  simp [Falsy, BitVec.ofNat, ← Fin.val_inj]
 
 instance : Decidable (Falsy v) := inferInstanceAs (Decidable (v = some 0))
 
@@ -89,57 +85,6 @@ inductive BigStep : Env → Stmt → Env → Prop where
     BigStep ρ (imp {while (~c) {~body}}) ρ
 
 attribute [simp] BigStep.skip
-
-theorem BigStep.unique : BigStep ρ s ρ' → BigStep ρ s ρ'' → ρ' = ρ'' := by
-  intro h1 h2
-  induction h1 generalizing ρ'' with
-  | «skip» => cases h2; rfl
-  | seq _s1 _s2 ih1 ih2 =>
-    cases h2 with
-    | seq s1' s2' =>
-      have := ih1 s1'
-      subst this
-      apply ih2 s2'
-  | assign isVal =>
-    cases h2 with
-    | assign isVal' =>
-      rw [isVal] at *
-      subst_eqs
-      rfl
-  | ifTrue isTrue _stepTrue ih =>
-    cases h2 with
-    | ifTrue isTrue' stepTrue' =>
-      exact ih stepTrue'
-    | ifFalse isFalse =>
-      have := isTrue.not_falsy
-      contradiction
-  | ifFalse isFalse _stepFalse ih =>
-    cases h2 with
-    | ifTrue isTrue' stepTrue' =>
-      have := isTrue'.not_falsy
-      contradiction
-    | ifFalse isFalse' stepFalse' =>
-      exact ih stepFalse'
-  | whileTrue isTrue _stepBody _stepLoop ihBody ihLoop =>
-    cases h2 with
-    | whileTrue isTrue' stepBody' stepLoop' =>
-      have := ihBody stepBody'
-      subst this
-      exact ihLoop stepLoop'
-    | whileFalse isFalse' =>
-      have := isTrue.not_falsy
-      contradiction
-  | whileFalse isFalse =>
-    cases h2 with
-    | whileTrue isTrue' stepBody' stepLoop' =>
-      have := isTrue'.not_falsy
-      contradiction
-    | whileFalse isFalse' =>
-      rfl
-
-
-
-
 
 /--
 `swap` terminates, and the resulting environment contains swapped inputs.
@@ -194,7 +139,6 @@ example : ∃ρ', BigStep (Env.init 0 |>.set "x" x |>.set "y" y) min ρ' ∧ if 
     . simp [Env.get, Env.set]
       intro; contradiction
 
-
 def loop := imp {while (1) {skip;}}
 
 /--
@@ -203,27 +147,14 @@ def loop := imp {while (1) {skip;}}
 theorem infinite_loop : ¬ BigStep ρ loop ρ' := by
   generalize h' : loop = l
   intro h
-  induction h with try (simp [loop, *] at *; done)
-  | whileTrue =>
+  induction h <;> try (simp [loop, *] at *; done)
+  case whileTrue =>
     simp [*]
-  | whileFalse cFalse =>
+  case whileFalse cFalse =>
     unfold loop at h'
     cases h'
-    cases cFalse
-
-def loopOf (s) := imp {while (1) {~s}}
-
-theorem infinite_loopOf : ¬ BigStep ρ (loopOf s) ρ' := by
-  generalize h' : loopOf s = l
-  intro h
-  induction h with try (simp [loopOf, *] at *; done)
-  | whileTrue =>
-    simp [*]
-  | whileFalse cFalse =>
-    unfold loopOf at h'
-    cases h'
-    cases cFalse
-
+    simp at cFalse
+    contradiction
 
 theorem optimize_ok : BigStep ρ s ρ' → BigStep ρ s.optimize ρ' := by
   intro h
@@ -292,173 +223,71 @@ theorem optimize_ok : BigStep ρ s ρ' → BigStep ρ s.optimize ρ' := by
         assumption
 
 
-inductive BigRes : Nat → Env → Stmt → Type where
-  | done (ρ' : Env) : BigStep ρ s ρ' → BigRes n ρ s
-  | noGas : BigRes n ρ s
-  | crash : ¬(∃ρ', BigStep ρ s ρ') →  BigRes n ρ s
-
-theorem BigStep.no_seq : ¬(∃ ρ', BigStep ρ (imp {~s1 ~s2}) ρ') ↔ ¬(∃ ρ' ρ'', BigStep ρ s1 ρ' ∧ BigStep ρ' s2 ρ'') := by
-  constructor
-  . intro no
-    intro ⟨ρ', ρ'', st1, st2⟩
-    apply no
-    constructor; constructor
-    exact st1
-    exact st2
-  . intro no
-    rintro ⟨ρ', ⟨st1, st2⟩⟩
-    apply no
-    constructor; constructor
-    constructor
-    . assumption
-    . assumption
-
-theorem BigStep.no_assign : ¬(∃ ρ', BigStep ρ (imp {~x := ~e;}) ρ') ↔ e.eval ρ = none := by
-  constructor
-  . intro noSteps
-    cases h : e.eval ρ <;> simp
-    apply noSteps
-    constructor
-    constructor
-    exact h
-  . intro isNone
-    intro h
-    rcases h with ⟨_, ⟨isSome⟩⟩
-    rw [isNone] at *; contradiction
-
-
-def run (ρ : Env) (s : Stmt) : (n : Nat) → BigRes n ρ s
-  | 0 => .noGas
-  | n + 1 =>
-    match s with
-    | imp {skip;} =>
-      .done ρ .skip
-    | imp {~s1 ~s2} =>
-      match run ρ s1 n with
-      | .done ρ' st1 =>
-        match run ρ' s2 n with
-        | .done ρ'' st2 => .done ρ'' (.seq st1 st2)
-        | .noGas => .noGas
-        | .crash no => .crash <| by
-          rw [BigStep.no_seq]
-          rintro ⟨ρ', ρ'', st1', st2'⟩
-          apply no
-          have := BigStep.unique st1 st1'
-          subst this
-          constructor; assumption
-      | .noGas => .noGas
-      | .crash no => .crash <| by
-        rw [BigStep.no_seq]
-        intro h
-        simp at h
-        apply no
-        rcases h with ⟨_, _, ⟨_, _⟩⟩
-        constructor; assumption
-    | imp {~x := ~e;} =>
-      match h : e.eval ρ with
-      | none => .crash <| by
-        rw [BigStep.no_assign]
-        simp [*]
-      | some v => .done _ (.assign h)
-    | imp {if (~c) {~s1} else {~s2}} =>
-      match h : c.eval ρ with
-      | none => .crash <| by
-        intro ⟨ρ', st⟩
-        cases st with
-        | ifTrue =>
-          simp [*] at *
-        | ifFalse =>
-          simp [*] at *
-      | some v =>
-        if h' : v = 0 then
-          match run ρ s2 n with
-          | .done ρ' step => .done ρ' (.ifFalse (by simp [h, h']) step)
-          | .noGas => .noGas
-          | .crash no => .crash <| by
-            intro ⟨ρ', st⟩
-            apply no
-            cases st with
-            | ifTrue isTrue step1 =>
-              have := isTrue.not_falsy
-              simp [*] at *
-            | ifFalse isFalse step2 =>
-              constructor; assumption
-        else
-          match run ρ s1 n with
-          | .done ρ' step => .done ρ' (.ifTrue (by simp [h, h']; assumption) step)
-          | .noGas => .noGas
-          | .crash no => .crash <| by
-            intro ⟨ρ', st⟩
-            apply no
-            cases st with
-            | ifTrue isTrue step1 =>
-              constructor; assumption
-            | ifFalse isFalse step2 =>
-              simp [Falsy, h, h'] at isFalse
-              contradiction
-    | imp {while (~c) {~s1}} =>
-      match h : c.eval ρ with
-      | none => .crash <| by
-        intro ⟨ρ', st⟩
-        cases st <;> simp [*] at *
-      | some v =>
-        if h' : v = 0 then
-          .done _ <| .whileFalse (by simp [*])
-        else
-          have truthy : Truthy (c.eval ρ) := by simp [*]; assumption
-          match run ρ s1 n with
-          | .done ρ' step =>
-            match run ρ' (imp {while (~c) {~s1}}) n with
-            | .done ρ'' step' =>
-              .done ρ'' (.whileTrue truthy step step')
-            | .noGas => .noGas
-            | .crash no =>
-              .crash <| by
-                intro ⟨ρ'', st⟩
-                cases st
-                . have := BigStep.unique step (by assumption)
-                  subst this
-                  apply no
-                  constructor; assumption
-                . simp [*] at *; contradiction
-          | .noGas => .noGas
-          | .crash no => .crash <| by
-            intro ⟨ρ', st⟩
-            cases st with
-            | whileFalse =>
-              simp [*] at *; contradiction
-            | whileTrue =>
-              apply no
-              constructor; assumption
-
-def run' (ρ : Env) (s : Stmt) : (n : Nat) → Option Env
+def run (ρ : Env) (s : Stmt) : Nat → Option Env
   | 0 => none
   | n + 1 =>
     match s with
     | imp {skip;} =>
       some ρ
     | imp {~s1 ~s2} => do
-      let ρ' ← run' ρ s1 n
-      run' ρ' s2 n
+      let ρ' ← run ρ s1 n
+      run ρ' s2 n
     | imp {~x := ~e;} => do
       let v ← e.eval ρ
       pure (ρ.set x v)
     | imp {if (~c) {~s1} else {~s2}} => do
       let v ← c.eval ρ
       if v = 0 then
-        run' ρ s2 n
+        run ρ s2 n
       else
-        run' ρ s1 n
+        run ρ s1 n
     | imp {while (~c) {~s1}} => do
       let v ← c.eval ρ
       if v = 0 then
         pure ρ
       else
-        let ρ' ← run' ρ s1 n
-        run' ρ' (imp {while (~c) {~s1}}) n
+        let ρ' ← run ρ s1 n
+        run ρ' (imp {while (~c) {~s1}}) n
 
-
-def terminatesWith (n : Nat) (ρ : Env) (s : Stmt) : Option Env :=
-  match run ρ s n with
-  | .done ρ' _ => some ρ'
-  | _ => none
+theorem run'_correct : run ρ s n = some ρ' → BigStep ρ s ρ' := by
+  intro term
+  induction ρ, s, n using run.induct generalizing ρ' <;> unfold run at term <;> simp_all
+  case case3 ρ n s1 s2 ih1 ih2 =>
+    let ⟨ρ'', ⟨st1, st2⟩⟩ := term
+    constructor
+    . apply ih1
+      apply st1
+    . apply ih2
+      apply st2
+  case case4 =>
+    let ⟨ρ'', ⟨evEq, setEq⟩⟩ := term
+    subst_eqs
+    constructor; assumption
+  case case5 ih1 ih2 =>
+    let ⟨v, ⟨evEq, step⟩⟩ := term
+    by_cases h : v = 0
+    . subst_eqs; simp at *
+      apply BigStep.ifFalse
+      . simp [Falsy, *]
+      . exact ih1 step
+    . subst_eqs; simp at *
+      apply BigStep.ifTrue
+      . simp [Truthy, *]
+      . simp [*] at step
+        apply ih2; assumption
+  case case6 ih1 ih2 =>
+    let ⟨v, ⟨evEq, step⟩⟩ := term
+    by_cases h : v = 0
+    . subst_eqs; simp at *
+      apply BigStep.whileFalse
+      simp [Falsy, *]
+    . subst_eqs; simp [*] at *
+      simp [h] at step
+      let ⟨ρ', ⟨oneStep, loopStep⟩⟩ := step
+      apply BigStep.whileTrue
+      . rw [evEq]
+        simp [*]
+      . apply ih1
+        exact oneStep
+      . apply ih2
+        exact loopStep
