Imp/Expr/Basic.lean
@@ -1,0 +1,23 @@
+namespace Imp.Expr
+
+inductive UnOp where
+  | neg
+  | not
+deriving Repr, DecidableEq
+
+inductive BinOp where
+  | plus | minus | times | div
+  | lsh | rsh
+  | band | bor
+  | and | or
+  | lt | le | eq
+deriving Repr, DecidableEq
+
+end Expr
+
+inductive Expr where
+  | const (i : BitVec 32)
+  | var (name : String)
+  | un (op : Expr.UnOp) (e : Expr)
+  | bin (op : Expr.BinOp) (e1 e2 : Expr)
+deriving Repr, DecidableEq
