Imp/Expr/Eval.lean
@@ -1,37 +1,50 @@
-import Imp.Expr
+import Imp.Expr.Basic
 
 open Lean
 
 namespace Imp
 
+/-- Values stored in memory - 32-bit integers -/
 abbrev Value := BitVec 32
 
+/-- An environment maps variables names to their values (no pointers) -/
 def Env := String → Value
 
 namespace Env
 
+/-- Set a value in an environment -/
 def set (x : String) (v : Value) (ρ : Env) : Env :=
   fun y => if x == y then v else ρ y
 
+/-- Look up a value in an environment -/
 def get (x : String) (ρ : Env) : Value :=
   ρ x
 
+/-- Initialize an environment, setting all uninitialized memory to `i` -/
 def init (i : Value) : Env := fun _ => i
+
+@[simp]
+theorem get_init : (Env.init v).get x = v := by rfl
+
+@[simp]
+theorem get_set_same {ρ : Env} : (ρ.set x v).get x = v := by
+  simp [get, set]
+
+@[simp]
+theorem get_set_different {ρ : Env} : x ≠ y → (ρ.set x v).get y = ρ.get y := by
+  intros
+  simp [get, set, *]
 
 end Env
 
 namespace Expr
 
-def freeVars : Expr → List String
-  | .const _ => []
-  | .var x => [x]
-  | .un _ e => e.freeVars
-  | .bin _ e1 e2 => e1.freeVars ++ e2.freeVars
-
+/-- Helper that implements unary operators -/
 def UnOp.apply : UnOp → Value → Option Value
   | .neg, x => some (- x)
   | .not, x => some (if x == 0 then 1 else 0)
 
+/-- Helper that implements binary operators -/
 def BinOp.apply : BinOp → Value → Value → Option Value
   | .plus, x, y => some (x + y)
   | .minus, x, y => some (x - y)
@@ -47,6 +60,11 @@ def BinOp.apply : BinOp → Value → Value → Option Value
   | .le, x, y => some (if x ≤ y then 1 else 0)
   | .lt, x, y => some (if x < y then 1 else 0)
 
+/--
+Evaluates an expression, finding the value if it has one.
+
+Expressions that divide by zero don't have values - the result is undefined.
+-/
 def eval (ρ : Env) : Expr → Option Value
   | .const i => some i
   | .var x => ρ.get x
