Imp/Expr/Syntax.lean
@@ -1,0 +1,108 @@
+import Lean.PrettyPrinter.Parenthesizer
+import Imp.Expr.Basic
+
+namespace Imp.Expr
+
+open Lean PrettyPrinter Parenthesizer
+
+declare_syntax_cat varname
+syntax ident : varname
+syntax:max "~" term:max : varname
+
+syntax "var " "{" varname "}" : term
+
+macro_rules
+  | `(var { $x:ident }) => `(term|$(quote x.getId.toString))
+  | `(var { ~$stx }) => pure stx
+
+declare_syntax_cat exp
+syntax varname : exp
+/-- Numeric constant -/
+syntax num : exp
+
+/-- Arithmetic complement -/
+syntax:75 "-" exp:75 : exp
+
+/-- Multiplication -/
+syntax:70 exp:70 " * " exp:71 : exp
+/-- Division -/
+syntax:70 exp:70 " / " exp:71 : exp
+
+/-- Addition -/
+syntax:65 exp:65 " + " exp:66 : exp
+/-- Subtraction -/
+syntax:65 exp:65 " - " exp:66 : exp
+
+syntax:55 exp:55 " <<< " exp:56 :exp
+syntax:55 exp:55 " >>> " exp:56 :exp
+
+/-- Boolean negation -/
+syntax:75 "!" exp:75 : exp
+/-- Less than -/
+syntax:50 exp:50 " < " exp:51 : exp
+/-- Less than or equal to -/
+syntax:50 exp:50 " ≤ " exp:51 : exp
+/-- Greater than or equal to -/
+syntax:50 exp:50 " ≥ " exp:51 : exp
+/-- Greater than -/
+syntax:50 exp:50 " > " exp:51 : exp
+/-- Equal -/
+syntax:45 exp:45 " == " exp:46 : exp
+
+syntax:40 exp:40 " &&& " exp:41 :exp
+syntax:40 exp:40 " ||| " exp:41 :exp
+
+/-- Boolean conjunction -/
+syntax:35 exp:35 " && " exp:36 : exp
+/-- Boolean disjunction -/
+syntax:35 exp:35 " || " exp:36 : exp
+
+/-- Parens -/
+syntax "(" exp ")" : exp
+
+/-- Escape to Lean -/
+syntax:max "~" term:max : exp
+
+syntax:min "expr " "{ " exp " }" : term
+
+open Lean in
+macro_rules
+  | `(expr{$x:ident}) => `(Expr.var $(quote x.getId.toString))
+  | `(expr{$n:num}) => `(Expr.const $(quote n.getNat))
+
+  | `(expr{-$e}) => `(Expr.un .neg (expr{$e}))
+  | `(expr{!$e}) => `(Expr.un .not (expr{$e}))
+
+  | `(expr{$e1 + $e2}) => `(Expr.bin .plus (expr{$e1}) (expr{$e2}))
+  | `(expr{$e1 * $e2}) => `(Expr.bin .times (expr{$e1}) (expr{$e2}))
+  | `(expr{$e1 - $e2}) => `(Expr.bin .minus (expr{$e1}) (expr{$e2}))
+  | `(expr{$e1 / $e2}) => `(Expr.bin .div (expr{$e1}) (expr{$e2}))
+
+  | `(expr{$e1 >>> $e2}) => `(Expr.bin .rsh (expr{$e1}) (expr{$e2}))
+  | `(expr{$e1 <<< $e2}) => `(Expr.bin .lsh (expr{$e1}) (expr{$e2}))
+  | `(expr{$e1 ||| $e2}) => `(Expr.bin .bor (expr{$e1}) (expr{$e2}))
+  | `(expr{$e1 &&& $e2}) => `(Expr.bin .band (expr{$e1}) (expr{$e2}))
+
+
+  | `(expr{$e1 && $e2}) => `(Expr.bin .and (expr{$e1}) (expr{$e2}))
+  | `(expr{$e1 || $e2}) => `(Expr.bin .or (expr{$e1}) (expr{$e2}))
+
+  | `(expr{$e1 < $e2}) => `(Expr.bin .lt (expr{$e1}) (expr{$e2}))
+  | `(expr{$e1 ≤ $e2}) => `(Expr.bin .le (expr{$e1}) (expr{$e2}))
+  | `(expr{$e1 == $e2}) => `(Expr.bin .eq (expr{$e1}) (expr{$e2}))
+  | `(expr{$e1 ≥ $e2}) => `(Expr.bin .le (expr{$e2}) (expr{$e1}))
+  | `(expr{$e1 > $e2}) => `(Expr.bin .lt (expr{$e2}) (expr{$e1}))
+  | `(expr{($e)}) => `(expr{$e})
+  | `(expr{~$stx}) => pure stx
+
+
+-- Shamelessly stolen from Lean's term parenthesizer - applies the precedence rules in the grammar
+-- to add parentheses as needed.
+@[category_parenthesizer exp]
+def exp.parenthesizer : CategoryParenthesizer | prec => do
+  maybeParenthesize `exp true wrapParens prec $
+    parenthesizeCategoryCore `exp prec
+where
+  wrapParens (stx : Syntax) : Syntax := Unhygienic.run do
+    let pstx ← `(($(⟨stx⟩)))
+    return pstx.raw.setInfo (SourceInfo.fromRef stx)
