README.md
@@ -3,12 +3,65 @@
 This repository contains materials used during Leo de Moura and David
 Thrane Christiansen's presentation at SSFT 2024.
 
+## Getting Ready
+
+To prepare for the Lean lectures, please install Lean using the
+[official instructions](https://lean-lang.org/lean4/doc/quickstart.html).
+This will set up everything you need for the summer school.
+
+If for some reason you can't follow these instructions, please make
+sure that the way you install Lean ends up with an installation of
+`elan`, the Lean toolchain version manager, rather than a specific
+version of Lean itself (e.g. from `nixpkgs`). The installation of elan
+worked if you can type `lean +4.7.0 --version` in your home directory,
+and it prints out `Lean (version 4.7.0, ...)`, and typing
+`lean +nightly-2024-05-19 --version` prints something like
+`Lean (version 4.9.0-nightly-2024-04-19, ...)`.
+
 ## First Lecture: Introduction to Lean
 
 This lecture is an introduction to writing programs, and proving them
-correct, in Lean. We interactively write a program that filters JSON
-objects, and prove it correct with respect to a number of
-specifications.
+correct, in Lean. After an introduction to Lean's syntax and the very
+basics of using its type theory as a logic, we interactively write a
+program that filters JSON objects, and prove it correct with respect
+to a number of specifications.
+
+The following files are part of the first lecture:
+
+ * `Intro.lean`
+ * The contents of the `tests/` directory
+ * `Main.lean` - the entry point for the JSON filter
+ * `Filter.lean` and the contents of `Filter/`:
+   - `Filter/List.lean` - a verified implementation of filtering lists
+   - `Filter/Array.lean` - a verified implementation of filtering arrays
+   - `Filter/Input.lean` - utilities for reading JSON (not part of
+     lectures)
+   - `Filter/Query.lean` - a query language (not part of lectures)
 
 
-## 
+
+## Second Lecture: 
+
+This lecture demonstrates how to use Lean for implementing languages
+and proving things about programs written in them. The programs are
+written in Imp, a minimal imperative language that features while
+loops, mutable variables, and conditionals.
+
+The following files are part of the second lecture:
+ * `Imp.lean` - the top-level module that exists to import the others
+ * `Imp/Expr.lean` - definition of an expression datatype and
+   convenient syntax for writing it
+ * `Imp/Expr/` - expressions and evaluation:
+   - `Imp/Expr/Eval.lean` - Evaluating expressions
+   - `Imp/Expr/Optimize.lean` - Constant-folding optimization of
+     expressions
+   - `Imp/Expr/Delab.lean` - Interactive display of expressions (not
+     part of lectures)
+ * `Imp/Stmt.lean` - definition of a statement datatype and convenient
+   syntax for writing it
+   - `Imp/Stmt/Optimize.lean` - Optimization of expressions
+   - `Imp/Stmt/BigStep.lean` - Operational semantics and proof that
+     optimization is correct
+   - `Imp/Stmt/Delab.lean` - Interactive display of statements (not
+     part of lectures)
+
